thys/Infinitary_Lambda_Calculus/ILC_affine.thy
@@ -8,9 +8,9 @@ begin
 (* *)
 
 lemma Tvars_dsset: "(FFVars t - dsset xs) \<inter> dsset xs = {}" "|FFVars t - dsset xs| <o |UNIV::ivar set|"
-apply auto using card_of_minus_bound iterm.set_bd_UNIV by blast
+apply auto using card_of_minus_bound ILterm.set_bd_UNIV by blast
 
-binder_inductive affine  :: "itrm \<Rightarrow> bool" where
+binder_inductive affine  :: "ilterm \<Rightarrow> bool" where
  iVar[simp,intro!]: "affine (iVar x)"
 |iLam: "affine e \<Longrightarrow> affine (iLam xs e)"
 |iApp:
@@ -35,7 +35,7 @@ binder_inductive affine  :: "itrm \<Rightarrow> bool" where
       subgoal apply(elim exE) subgoal for e xs
         apply(rule exI[of _ "irrename \<sigma> e"])
         apply(rule exI[of _ "dsmap \<sigma> xs"])
-        apply (simp add: iterm.rrename_comps)
+        apply (simp add: ILterm.rrename_comps)
         done
       done
     done
@@ -44,7 +44,7 @@ binder_inductive affine  :: "itrm \<Rightarrow> bool" where
       subgoal apply(elim exE) subgoal for e1 es2
         apply(rule exI[of _ "irrename \<sigma> e1"])
         apply(rule exI[of _ "smap (irrename \<sigma>) es2"])
-        apply (fastforce simp add: iterm.rrename_comps)
+        apply (fastforce simp add: ILterm.rrename_comps)
         done
       done
     done
@@ -104,7 +104,7 @@ assumes "affine (iLam xs e)"
 shows "affine e"
 proof-
   obtain xs' e' where 0: "iLam xs e = iLam xs' e'" and "affine e'"
-  using assms by (smt (verit, del_insts) affine.cases iterm.distinct(2) iterm.distinct(4))
+  using assms by (smt (verit, del_insts) affine.cases ILterm.distinct(2) ILterm.distinct(4))
   thus ?thesis using 0 unfolding iLam_inject
   by (metis iLam_inject affine.equiv)
 qed
@@ -119,17 +119,17 @@ using affine.simps affine_iLam_case by blast
 lemma tvsubst_affine':
 assumes f: "|SSupp f| <o |UNIV::ivar set|" and af: "\<And>x. affine (f x)"
 and fv: "\<And>x y. x \<noteq> y \<Longrightarrow> FFVars (f x) \<inter> FFVars (f y) = {}"
-and r: "affine (e::itrm)"
+and r: "affine (e::ilterm)"
 shows "affine (itvsubst f e)"
 using r proof (binder_induction e avoiding: "IImsupp f" rule: affine.strong_induct)
   case (iLam ea xs)
-  show ?case using iLam apply(subst iterm.subst)
+  show ?case using iLam apply(subst ILterm.subst)
       subgoal using f by auto
       subgoal by auto
       subgoal apply(rule affine.iLam) by auto .
 next
   case (iApp e1 es2)
-  then show ?case apply(subst iterm.subst)
+  then show ?case apply(subst ILterm.subst)
       subgoal using f by auto
       subgoal apply(rule affine.iApp) using fv f
       by auto (metis Int_emptyD)+ .
@@ -141,7 +141,7 @@ not strong enough to instantiate to imakeSubst... *)
 lemma tvsubst_affine:
 assumes f: "|SSupp f| <o |UNIV::ivar set|" and af: "\<And>x. affine (f x)"
 and fv: "\<And>x y. {x,y} \<subseteq> FFVars e \<Longrightarrow> x \<noteq> y \<Longrightarrow> FFVars (f x) \<inter> FFVars (f y) = {}"
-and r: "affine (e::itrm)"
+and r: "affine (e::ilterm)"
 shows "affine (itvsubst f e)"
 proof-
   obtain xs and x::ivar where x: "x \<in> dsset xs"
@@ -150,7 +150,7 @@ proof-
   have t: "FFVars t = {}" "affine t" unfolding t_def using x by (auto intro: affine.intros)
 
   have fve: "\<And>e. |FFVars e| <o |UNIV::ivar set|"
-    by (simp add: iterm.set_bd_UNIV)
+    by (simp add: ILterm.set_bd_UNIV)
 
   have "|\<Union> ((FFVars o f) ` (FFVars e))| \<le>o |Sigma (FFVars e) (FFVars o f)|"
   by (rule card_of_UNION_Sigma)
@@ -190,7 +190,7 @@ shows "affine (itvsubst (imkSubst xs es) e)"
 apply(rule tvsubst_affine)
 using assms apply auto
   apply (simp add: imkSubst_def)
-  by (metis Int_emptyD dtheN imkSubst_def iterm.set(1) singletonD snth_sset)
+  by (metis Int_emptyD dtheN imkSubst_def ILterm.set(1) singletonD snth_sset)
 
 lemma imkSubst_affine_strong:
 assumes r: "affine e" and
@@ -200,7 +200,7 @@ shows "affine (itvsubst (imkSubst xs es) e)"
 apply(rule tvsubst_affine)
 using assms apply auto
   apply (simp add: imkSubst_def)
-  by (smt (verit, best) IntI disjoint_insert(2) dtheN imkSubst_def in_mono iterm.set(1)
+  by (smt (verit, best) IntI disjoint_insert(2) dtheN imkSubst_def in_mono ILterm.set(1)
   mk_disjoint_insert singletonD snth_sset)
 
 end
